% !TEX root = main.tex
\section{Transforming Subsequence Searching\\ to Lookup Arguments}
\begin{frame}{Recalling Constraints}
	We would like to construct the sequence $(p_j)_{j \in [0, N]}$ with $p_0 = 0$ satisfying three constraints:
	\begin{itemize}
		\item Constraint 1: $p_j = p_{j - 1}$ if $p_{j - 1} = N$;\\
		\item Constraint 2: $p_j = p_{j - 1} + 1$ if $s_{p_{j - 1} + 1} = t_j$; and\\
		\item Constraint 3: $p_j = p_{j - 1}$, otherwise (when $s_{p_{j - 1} + 1} \not= t_j$).
	\end{itemize}
	
	\textbf{Handling Constraint 1.} Appending $\perp$ to the end of $\bs$, i.e.,
	\begin{equation*}
		\bs_\perp = (\bs\Vert\!\perp) = (s_1, \dots, s_n, \perp).
	\end{equation*}
	$\Rightarrow$ Constraint 1 is implied by constraint 3 since $\perp \not= v~\forall v \in \Sigma$.
\end{frame}
\begin{frame}{Handling Constraints 2 and 3}
	\textbf{From constraint 2:} $p_j = p_{j - 1} + 1$ if $s_{p_{j - 1} + 1} = t_j$.
	
	\textbf{From constraint 3:} $p_j = p_{j - 1}$ if $s_{p_{j - 1} + 1} \not= t_j$.
	
	We have the equivalences
	\begin{equation}\label{equation:system-of-equivalences-for-constraints-2-and-3}
		\begin{cases}
			p_j - p_{j - 1} = 1 \iff s_{p_{j - 1} + 1} = t_j,\\ 
			p_j - p_{j - 1} = 0 \iff s_{p_{j - 1} + 1} \not= t_j.
		\end{cases}
	\end{equation}
	
	Define $\enc(\bs_\perp)  = \{(c, \ell, v) \in \{0,1\}\times[n+1]\times\Sigma\cup\{\perp\} : c = (s_\ell = v)\}$.
	
	Then,
	$
		\eqref{equation:system-of-equivalences-for-constraints-2-and-3} \iff (p_j - p_{j - 1}, p_{j - 1} + 1, t_j) \in \enc(\bs_\perp).
	$
	
	\pause
	\begin{center}
		\textbf{How to guarantee well-formedness of $\enc(\bs_\perp)$?}
	\end{center}
\end{frame}

\begin{frame}{An observation from $\enc(\bs_\perp)$}
	$\enc(\bs_\perp)  = \{(c, \ell, v) \in \{0,1\}\times[n+1]\times\Sigma\cup\{\perp\} : c = (s_\ell = v)\}$.
	
	$\size{\enc(\bs_\perp)} = (n + 1)\cdot (\size{\Sigma} + 1) = \BigO(n \times \size{\Sigma})$ which is inefficient.
	
	\pause
	\begin{center}
		\textbf{Is there any alternative way?}
	\end{center}
\end{frame}

\begin{frame}{An Alternative Approach}
	%Recall from \eqref{equation:system-of-equivalences-for-constraints-2-and-3} 
	\begin{equation*}
		\begin{cases}
			p_j - p_{j - 1} = 1 \iff s_{p_{j - 1} + 1} = t_j,\\ 
			p_j - p_{j - 1} = 0 \iff s_{p_{j - 1} + 1} \not= t_j.
		\end{cases}
	\end{equation*}
	
	Let $v_j := s_{p_{j - 1} + 1}$. Well-formedness of $(v_j)_{j \in [N]}$ is guaranteed by
	\begin{equation*}
		\{(p_{j - 1} + 1, v_j)\}_{j \in [N]} \subseteq \{(j, s_j)\}_{j \in [n + 1]}.
	\end{equation*}
	
	Then, to determine $ c_j = (s_{p_{j - 1} + 1} = t_j)$, we instead determine whether $c_j = (v_j = t_j)$. One hence checks whether $p_j - p_{j - 1} = c_j$.
	
	$
		\begin{cases}
			v_j = t_j \iff v_j - t_j = 0,\\ v_j\not=t_j\iff v_j - t_j \in [-\size{\Sigma}, \size{\Sigma}]\setminus\{0\}
		\end{cases}
	$ 
	
	$
		\Rightarrow \{(p_j - p_{j - 1}, v_j - t_j)\}_{j \in [N]} \subseteq \{(0, i)\}_{i \in [-\size{\Sigma}, \size{\Sigma}]\setminus\{0\}} \cup \{(1, 0)\}.
	$
\end{frame}

\begin{frame}{Final Theorem}
	$\bs$ is a subsequence (respectively, non-subsequence) of $\bt$  iff there exist $s_{n+1}$, $(p_j)_{j \in [0, N]}$, with $p_0=0$ by default,  and $(v_j)_{j \in [N]}$ s.t.
	\begin{equation*}%\label{equation:constraints-for-wellformedness-of-b-in-single-subsequence-argument}
		\begin{cases}
			\{s_j\}_{j \in [n]} \subseteq \Sigma,\quad s_{n+1} = \perp,\quad \{t_j\}_{j \in [N]} \subseteq \Sigma,\\
			\{(p_{j - 1} + 1, v_j)\}_{j \in [N]} \subseteq \{(j, s_j)\}_{j \in [n+1]},\\
			\{(p_j - p_{j - 1}, t_j - v_j)\}_{j \in [N]} \subseteq \{(0,i)\}_{i \in [-\size{\Sigma}, \size{\Sigma}]\setminus\{0\}} \cup \{(1, 0)\},
		\end{cases}
	\end{equation*}
	and $p_N < n$ (respectively, $p_N = n$).
\end{frame}